attempt to update iris and fix associated errors

theories/iris.v
@@ -5,22 +5,658 @@ From mathcomp Require Import ssreflect ssrbool eqtype seq.
 
 (* There is a conflict between ssrnat and Iris language. *)
 (* Also a conflict between ssrnat and stdpp on the notation .* *)
-From iris.program_logic Require Import ectx_lifting total_ectx_lifting.
-From iris.program_logic Require Import language ectx_language ectxi_language.
 
 Set Implicit Arguments.
 Unset Strict Implicit.
 Unset Printing Implicit Defensive.
 
-Require Import common operations_iris datatypes_iris datatypes_properties_iris.
-Require Import iris_locations iris_base iris_opsem.
-
 From stdpp Require Import gmap.
-From iris.proofmode Require Import tactics.
 From iris.algebra Require Import auth.
 From iris.bi.lib Require Import fractional.
+From iris.proofmode Require Import tactics.
 From iris.base_logic.lib Require Export gen_heap proph_map gen_inv_heap.
 From iris.program_logic Require Export weakestpre total_weakestpre.
+From iris.program_logic Require Import language.
+
+Require Import common operations_iris datatypes_iris datatypes_properties_iris.
+Require Import list_extra.
+Require Import iris_locations.
+
+Definition iris_expr := host_expr.
+Definition iris_val := host_value.
+(* Use gmap to specify the host variable store instead. *)
+Definition host_state := gmap id iris_val.
+Definition state : Type := host_state * store_record * list host_value.
+Definition observation := unit. (* TODO: ??? *)
+
+Definition of_val (v : iris_val) : iris_expr := HE_value v.
+
+Fixpoint to_val (e : iris_expr) : option iris_val :=
+  match e with
+  | HE_value v => Some v
+  | _ => None
+  end.
+  
+(* https://softwarefoundations.cis.upenn.edu/qc-current/Typeclasses.html *)
+Global Instance val_eq_dec : EqDecision iris_val.
+Proof.
+  decidable_equality.
+Defined.
+
+Lemma of_to_val e v : to_val e = Some v → of_val v = e.
+Proof.
+  destruct e => //=.
+  move => H. by inversion H.
+Qed.
+
+Inductive reduce_simple : list administrative_instruction -> list administrative_instruction -> Prop :=
+
+(** unop **)
+  | rs_unop : forall v op t,
+    reduce_simple [::AI_basic (BI_const v); AI_basic (BI_unop t op)] [::AI_basic (BI_const (@app_unop op v))]
+                   
+(** binop **)
+  | rs_binop_success : forall v1 v2 v op t,
+    app_binop op v1 v2 = Some v ->
+    reduce_simple [::AI_basic (BI_const v1); AI_basic (BI_const v2); AI_basic (BI_binop t op)] [::AI_basic (BI_const v)]
+  | rs_binop_failure : forall v1 v2 op t,
+    app_binop op v1 v2 = None ->
+    reduce_simple [::AI_basic (BI_const v1); AI_basic (BI_const v2); AI_basic (BI_binop t op)] [::AI_trap]
+                  
+  (** testops **)
+  | rs_testop_i32 :
+    forall c testop,
+    reduce_simple [::AI_basic (BI_const (VAL_int32 c)); AI_basic (BI_testop T_i32 testop)] [::AI_basic (BI_const (VAL_int32 (wasm_bool (@app_testop_i i32t testop c))))]
+  | rs_testop_i64 :
+    forall c testop,
+    reduce_simple [::AI_basic (BI_const (VAL_int64 c)); AI_basic (BI_testop T_i64 testop)] [::AI_basic (BI_const (VAL_int32 (wasm_bool (@app_testop_i i64t testop c))))]
+
+  (** relops **)
+  | rs_relop: forall v1 v2 t op,
+    reduce_simple [::AI_basic (BI_const v1); AI_basic (BI_const v2); AI_basic (BI_relop t op)] [::AI_basic (BI_const (VAL_int32 (wasm_bool (app_relop op v1 v2))))]
+                    
+  (** convert and reinterpret **)
+  | rs_convert_success :
+    forall t1 t2 v v' sx,
+    types_agree t1 v ->
+    cvt t2 sx v = Some v' ->
+    reduce_simple [::AI_basic (BI_const v); AI_basic (BI_cvtop t2 CVO_convert t1 sx)] [::AI_basic (BI_const v')]
+  | rs_convert_failure :
+    forall t1 t2 v sx,
+    types_agree t1 v ->
+    cvt t2 sx v = None ->
+    reduce_simple [::AI_basic (BI_const v); AI_basic (BI_cvtop t2 CVO_convert t1 sx)] [::AI_trap]
+  | rs_reinterpret :
+    forall t1 t2 v,
+    types_agree t1 v ->
+    reduce_simple [::AI_basic (BI_const v); AI_basic (BI_cvtop t2 CVO_reinterpret t1 None)] [::AI_basic (BI_const (wasm_deserialise (bits v) t2))]
+
+  (** control-flow operations **)
+  | rs_unreachable :
+    reduce_simple [::AI_basic BI_unreachable] [::AI_trap]
+  | rs_nop :
+    reduce_simple [::AI_basic BI_nop] [::]
+  | rs_drop :
+    forall v,
+    reduce_simple [::AI_basic (BI_const v); AI_basic BI_drop] [::]
+  | rs_select_false :
+    forall n v1 v2,
+    n = Wasm_int.int_zero i32m ->
+    reduce_simple [::AI_basic (BI_const v1); AI_basic (BI_const v2); AI_basic (BI_const (VAL_int32 n)); AI_basic BI_select] [::AI_basic (BI_const v2)]
+  | rs_select_true :
+    forall n v1 v2,
+    n <> Wasm_int.int_zero i32m ->
+    reduce_simple [::AI_basic (BI_const v1); AI_basic (BI_const v2); AI_basic (BI_const (VAL_int32 n)); AI_basic BI_select] [::AI_basic (BI_const v1)]
+  | rs_block :
+      forall vs es n m t1s t2s,
+        const_list vs ->
+        length vs = n ->
+        length t1s = n ->
+        length t2s = m ->
+        reduce_simple (vs ++ [::AI_basic (BI_block (Tf t1s t2s) es)]) [::AI_label m [::] (vs ++ to_e_list es)]
+  | rs_loop :
+      forall vs es n m t1s t2s,
+        const_list vs ->
+        length vs = n ->
+        length t1s = n ->
+        length t2s = m ->
+        reduce_simple (vs ++ [::AI_basic (BI_loop (Tf t1s t2s) es)]) [::AI_label n [::AI_basic (BI_loop (Tf t1s t2s) es)] (vs ++ to_e_list es)]
+  | rs_if_false :
+      forall n tf e1s e2s,
+        n = Wasm_int.int_zero i32m ->
+        reduce_simple ([::AI_basic (BI_const (VAL_int32 n)); AI_basic (BI_if tf e1s e2s)]) [::AI_basic (BI_block tf e2s)]
+  | rs_if_true :
+      forall n tf e1s e2s,
+        n <> Wasm_int.int_zero i32m ->
+        reduce_simple ([::AI_basic (BI_const (VAL_int32 n)); AI_basic (BI_if tf e1s e2s)]) [::AI_basic (BI_block tf e1s)]
+  | rs_label_const :
+      forall n es vs,
+        const_list vs ->
+        reduce_simple [::AI_label n es vs] vs
+  | rs_label_trap :
+      forall n es,
+        reduce_simple [::AI_label n es [::AI_trap]] [::AI_trap]
+  | rs_br :
+      forall n vs es i LI lh,
+        const_list vs ->
+        length vs = n ->
+        lfilled i lh (vs ++ [::AI_basic (BI_br i)]) LI ->
+        reduce_simple [::AI_label n es LI] (vs ++ es)
+  | rs_br_if_false :
+      forall n i,
+        n = Wasm_int.int_zero i32m ->
+        reduce_simple [::AI_basic (BI_const (VAL_int32 n)); AI_basic (BI_br_if i)] [::]
+  | rs_br_if_true :
+      forall n i,
+        n <> Wasm_int.int_zero i32m ->
+        reduce_simple [::AI_basic (BI_const (VAL_int32 n)); AI_basic (BI_br_if i)] [::AI_basic (BI_br i)]
+  | rs_br_table : (* ??? *)
+      forall iss c i j,
+        length iss > Wasm_int.nat_of_uint i32m c ->
+        List.nth_error iss (Wasm_int.nat_of_uint i32m c) = Some j ->
+        reduce_simple [::AI_basic (BI_const (VAL_int32 c)); AI_basic (BI_br_table iss i)] [::AI_basic (BI_br j)]
+  | rs_br_table_length :
+      forall iss c i,
+        length iss <= (Wasm_int.nat_of_uint i32m c) ->
+        reduce_simple [::AI_basic (BI_const (VAL_int32 c)); AI_basic (BI_br_table iss i)] [::AI_basic (BI_br i)]
+  | rs_local_const :
+      forall es n f,
+        const_list es ->
+        length es = n ->
+        reduce_simple [::AI_local n f es] es
+  | rs_local_trap :
+      forall n f,
+        reduce_simple [::AI_local n f [::AI_trap]] [::AI_trap]
+  | rs_return : (* ??? *)
+      forall n i vs es lh f,
+        const_list vs ->
+        length vs = n ->
+        lfilled i lh (vs ++ [::AI_basic BI_return]) es ->
+        reduce_simple [::AI_local n f es] vs
+  | rs_tee_local :
+      forall i v,
+        is_const v ->
+        reduce_simple [::v; AI_basic (BI_tee_local i)] [::v; v; AI_basic (BI_set_local i)]
+  | rs_trap :
+      forall es lh,
+        es <> [::AI_trap] ->
+        lfilled 0 lh [::AI_trap] es ->
+        reduce_simple es [::AI_trap]
+.
+
+Inductive pure_reduce : host_state -> store_record -> list host_value -> host_expr ->
+                        host_state -> store_record -> list host_value -> host_expr -> Prop :=
+  (* TODO: basic exprs -- arith ops, list ops left *)
+  | pr_getglobal:
+      forall hs s locs id hv ,
+      (* Upd: ok it does make sense for the lookup result to carry a double Some, since
+           gmap lookup itself returns an option.
+
+         After some thoughts, this double option should be allowing us a way to know that 
+           a memory is actually freed -- so we can distinguish between what we don't know and
+           what we know to be non-existent.
+
+         Also, the error message from the Lookup typeclass doesn't point to a specific line.. *)
+      hs !! id = Some hv ->
+      pure_reduce hs s locs (HE_getglobal id) hs s locs (HE_value hv)
+  | pr_getglobal_trap:
+    forall hs s locs id,
+      hs !! id = None ->
+      pure_reduce hs s locs (HE_getglobal id) hs s locs (HE_value HV_trap)
+  | pr_setglobal_value:
+    forall hs s locs id hv hs',
+      hv <> HV_trap ->
+      hs' = <[id := hv]> hs ->
+      pure_reduce hs s locs (HE_setglobal id (HE_value hv)) hs' s locs (HE_value hv)
+  | pr_setglobal_trap:
+    forall hs s locs id,
+      pure_reduce hs s locs (HE_setglobal id (HE_value HV_trap)) hs s locs (HE_value HV_trap)
+  | pr_setglobal_step:
+    forall hs s locs e hs' s' locs' e' id,
+      pure_reduce hs s locs e hs' s' locs' e' ->
+      pure_reduce hs s locs (HE_setglobal id e) hs' s' locs' (HE_setglobal id e')
+  | pr_getlocal:
+    forall hs s locs n hv,
+      locs !! (nat_of_N n) = Some hv ->
+      pure_reduce hs s locs (HE_getlocal n) hs s locs (HE_value hv)
+  | pr_getlocal_trap:
+    forall hs s locs n,
+      locs !! (nat_of_N n) = None ->
+      pure_reduce hs s locs (HE_getlocal n) hs s locs (HE_value HV_trap)
+  | pr_setlocal:
+    forall hs s locs n id locs' hv,
+      hs !! id = Some hv ->
+      (nat_of_N n) < length locs ->
+      locs' = list_insert (N.to_nat n) hv locs ->
+      pure_reduce hs s locs (HE_setlocal n id) hs s locs' (HE_value hv)
+  | pr_setlocal_trap1:
+    forall hs s locs n id,
+      hs !! id = None ->
+      pure_reduce hs s locs (HE_setlocal n id) hs s locs (HE_value HV_trap)
+  | pr_setlocal_trap2:
+    forall hs s locs n id hv,
+      hs !! id = Some hv ->
+      (nat_of_N n) >= length locs ->
+      pure_reduce hs s locs (HE_setlocal n id) hs s locs (HE_value HV_trap)
+  | pr_if_true:
+    forall hs s locs id e1 e2 hv,
+      hs !! id = Some hv ->
+      hv <> HV_wasm_value (VAL_int32 (Wasm_int.int_zero i32m)) ->
+      hv ≠ HV_trap ->
+      pure_reduce hs s locs (HE_if id e1 e2) hs s locs e1
+  | pr_if_false: 
+    forall hs s locs id e1 e2 hv,
+      hs !! id = Some hv ->
+      hv = HV_wasm_value (VAL_int32 (Wasm_int.int_zero i32m)) ->
+      pure_reduce hs s locs (HE_if id e1 e2) hs s locs e2
+  | pr_if_trap: 
+    forall hs s locs id e1 e2 hv,
+      hs !! id = Some hv ->
+      hv = HV_trap ->
+      pure_reduce hs s locs (HE_if id e1 e2) hs s locs (HE_value HV_trap)
+  | pr_if_none: 
+    forall hs s locs id e1 e2,
+      hs !! id = None ->
+      pure_reduce hs s locs (HE_if id e1 e2) hs s locs (HE_value HV_trap)
+  | pr_while:
+    forall hs s locs id e,
+      pure_reduce hs s locs (HE_while id e) hs s locs (HE_if id (HE_seq e (HE_while id e)) (HE_value (HV_wasm_value (VAL_int32 (Wasm_int.int_zero i32m)))))
+  (* record exprs *)
+  | pr_new_rec:
+    forall hs s locs kip hvs kvp,
+      list_extra.those (fmap (fun id => hs !! id) kip.*2) = Some hvs ->
+      zip kip.*1 hvs = kvp ->
+      pure_reduce hs s locs (HE_new_rec kip) hs s locs (HE_value (HV_record kvp))
+  | pr_new_rec_trap:
+    forall hs s locs kip,
+      list_extra.those (fmap (fun id => hs !! id) kip.*2) = None ->
+      pure_reduce hs s locs (HE_new_rec kip) hs s locs (HE_value HV_trap)
+  | pr_getfield:
+    forall hs s locs id fname kvp hv,
+      hs !! id = Some (HV_record kvp) ->
+      lookup_kvp kvp fname = Some hv -> 
+      pure_reduce hs s locs (HE_get_field id fname) hs s locs (HE_value hv)
+  | pr_getfield_trap1:
+    forall hs s locs id fname kvp,
+      hs !! id = Some (HV_record kvp) ->
+      lookup_kvp kvp fname = None ->
+      pure_reduce hs s locs (HE_get_field id fname) hs s locs (HE_value HV_trap)
+  | pr_getfield_trap2:
+    forall hs s locs id fname hv,
+      hs !! id = Some hv ->
+      host_typeof hv <> Some HT_record ->
+      pure_reduce hs s locs (HE_get_field id fname) hs s locs (HE_value HV_trap)
+  | pr_getfield_trap3:
+    forall hs s locs id fname,
+      hs !! id = None ->
+      pure_reduce hs s locs (HE_get_field id fname) hs s locs (HE_value HV_trap)
+  (* function exprs *)
+  | pr_new_host_func:
+    forall hs s locs htf locsn e s' n,
+      s' = {|s_funcs := s.(s_funcs) ++ [::datatypes_iris.FC_func_host htf locsn e]; s_tables := s.(s_tables); s_mems := s.(s_mems); s_globals := s.(s_globals) |} ->
+      n = length s.(s_funcs) ->
+      pure_reduce hs s locs (HE_new_host_func htf (N_of_nat locsn) e) hs s' locs (HE_value (HV_wov (WOV_funcref (Mk_funcidx n))))
+  | pr_call_wasm:
+    forall hs s ids cl id i j vts bes tf vs tn tm vars locs,
+      hs !! id = Some (HV_wov (WOV_funcref (Mk_funcidx i))) ->
+      s.(s_funcs) !! i = Some cl ->
+      cl = FC_func_native j tf vts bes ->
+      tf = Tf tn tm ->
+      list_extra.those (fmap (fun id => hs !! id) ids) = Some vars ->
+      list_host_value_to_wasm vars = Some vs ->
+      tn = fmap typeof vs ->
+      pure_reduce hs s locs (HE_call id ids) hs s locs (HE_wasm_frame ((v_to_e_list vs) ++ [::AI_invoke i]))
+  | pr_call_trap1:
+    forall hs s locs id ids,
+      hs !! id = None ->
+      pure_reduce hs s locs (HE_call id ids) hs s locs (HE_value HV_trap)
+  | pr_call_trap2:
+    forall hs s locs id ids v,
+      hs !! id = Some v ->
+      is_funcref v = false ->
+      pure_reduce hs s locs (HE_call id ids) hs s locs (HE_value HV_trap)
+  | pr_call_trap3:
+    forall hs s locs id ids i,
+      hs !! id = Some (HV_wov (WOV_funcref (Mk_funcidx i))) ->
+      s.(s_funcs) !! i = None ->
+      pure_reduce hs s locs (HE_call id ids) hs s locs (HE_value HV_trap)  
+  | pr_call_trap4:
+    forall hs s locs id ids,
+      list_extra.those (fmap (fun id => hs !! id) ids) = None ->
+      pure_reduce hs s locs (HE_call id ids) hs s locs (HE_value HV_trap)
+  | pr_call_wasm_trap1:
+    forall hs s locs id ids i cl j tf vts bes vars tn tm,
+      hs !! id = Some (HV_wov (WOV_funcref (Mk_funcidx i))) ->
+      s.(s_funcs) !! i = Some cl ->
+      cl = FC_func_native j tf vts bes ->
+      tf = Tf tn tm ->
+      list_extra.those (fmap (fun id => hs !! id) ids) = Some vars ->
+      list_host_value_to_wasm vars = None ->
+      pure_reduce hs s locs (HE_call id ids) hs s locs (HE_value HV_trap)  
+  | pr_call_wasm_trap2:
+    forall hs s locs id ids i cl j tf vts bes vars tn tm vs,
+      hs !! id = Some (HV_wov (WOV_funcref (Mk_funcidx i))) ->
+      s.(s_funcs) !! i = Some cl ->
+      cl = FC_func_native j tf vts bes ->
+      tf = Tf tn tm ->
+      list_extra.those (fmap (fun id => hs !! id) ids) = Some vars ->
+      list_host_value_to_wasm vars = Some vs ->
+      tn <> fmap typeof vs ->
+      pure_reduce hs s locs (HE_call id ids) hs s locs (HE_value HV_trap)  
+  | pr_call_host:
+    forall hs s ids cl id i n e tf tn tm vars vs locs,
+      hs !! id = Some (HV_wov (WOV_funcref (Mk_funcidx i))) ->
+      s.(s_funcs) !! i = Some cl ->
+      cl = FC_func_host tf n e ->
+      tf = Tf tn tm ->
+      list_extra.those (map (fun id => hs !! id) ids) = Some vars ->
+      list_host_value_to_wasm vars = Some vs -> (* TODO: change this to explicit casts, then add a trap case. *)
+      tn = fmap typeof vs ->
+      pure_reduce hs s locs (HE_call id ids) hs s locs (HE_wasm_frame ((v_to_e_list vs) ++ [::AI_invoke i]))
+  (* wasm state exprs *)
+  | pr_table_create:
+    forall hs s locs s' tab len n,
+      tab = create_table len ->
+      s' = {|s_funcs := s.(s_funcs); s_tables := s.(s_tables) ++ [::tab]; s_mems := s.(s_mems); s_globals := s.(s_globals) |} ->
+      n = length s.(s_tables) ->
+      pure_reduce hs s locs (HE_wasm_table_create len) hs s' locs (HE_value (HV_wov (WOV_tableref (Mk_tableidx n))))
+  | pr_table_set:
+    forall hs s locs idt n id v tn tab tab' s' fn,
+      hs !! idt = Some (HV_wov (WOV_tableref (Mk_tableidx tn))) ->
+      s.(s_tables) !! tn = Some tab ->
+      hs !! id = Some v ->
+      v = HV_wov (WOV_funcref (Mk_funcidx fn)) ->
+      tab' = {|table_data := list_insert n (Some fn) tab.(table_data); table_max_opt := tab.(table_max_opt) |} ->
+      s' = {|s_funcs := s.(s_funcs); s_tables := list_insert tn tab' s.(s_tables); s_mems := s.(s_mems); s_globals := s.(s_globals) |} ->
+      pure_reduce hs s locs (HE_wasm_table_set idt (N_of_nat n) id) hs s' locs (HE_value v)
+  | pr_table_get:
+    forall hs s locs idt n tn tab fn,
+      hs !! idt = Some (HV_wov (WOV_tableref (Mk_tableidx tn))) ->
+      s.(s_tables) !! tn = Some tab ->
+      tab.(table_data) !! n = Some (Some fn) ->
+      pure_reduce hs s locs (HE_wasm_table_get idt (N_of_nat n)) hs s locs (HE_value (HV_wov (WOV_funcref (Mk_funcidx fn))))
+  | pr_memory_create:
+    forall hs s locs s' sz sz_lim n,
+      s' = {|s_funcs := s.(s_funcs); s_tables := s.(s_tables); s_mems := s.(s_mems) ++ [::create_memory sz sz_lim]; s_globals := s.(s_globals) |} ->
+      n = length s.(s_mems) ->
+      pure_reduce hs s locs (HE_wasm_memory_create sz sz_lim) hs s' locs (HE_value (HV_wov (WOV_memoryref (Mk_memidx n))))
+  | pr_memory_set:
+    forall hs s locs idm n id md' mn m m' s' b,
+      hs !! idm = Some (HV_wov (WOV_memoryref (Mk_memidx mn))) ->
+      s.(s_mems) !! mn = Some m ->
+      hs !! id = Some (HV_byte b) ->
+      memory_list.mem_update n b m.(mem_data) = Some md' ->
+      m' = {|mem_data := md'; mem_max_opt := m.(mem_max_opt) |} ->
+      s' = {|s_funcs := s.(s_funcs); s_tables := s.(s_tables); s_mems := list_insert mn m' s.(s_mems); s_globals := s.(s_globals) |} ->
+      pure_reduce hs s locs (HE_wasm_memory_set idm n id) hs s' locs (HE_value (HV_byte b))
+  | pr_memory_get:
+    forall hs s locs idm n b m mn,
+      hs !! idm = Some (HV_wov (WOV_memoryref (Mk_memidx mn))) ->
+      s.(s_mems) !! mn = Some m ->
+      memory_list.mem_lookup n m.(mem_data) = Some b ->
+      pure_reduce hs s locs (HE_wasm_memory_get idm n) hs s locs (HE_value (HV_byte b))
+  | pr_memory_grow:
+    forall hs s s' locs idm n m m' mn,
+      hs !! idm = Some (HV_wov (WOV_memoryref (Mk_memidx mn))) ->
+      s.(s_mems) !! mn = Some m ->
+      mem_grow m n = Some m' ->
+      s' = {|s_funcs := s.(s_funcs); s_tables := s.(s_tables); s_mems := list_insert mn m' s.(s_mems); s_globals := s.(s_globals) |} ->
+      pure_reduce hs s locs (HE_wasm_memory_grow idm n) hs s' locs (HE_value (HV_wasm_value (VAL_int32 (Wasm_int.int_of_Z i32m (Z.of_N (mem_size m'))))))
+  | pr_globals_create:
+    forall hs s locs s' g n,
+      s' = {|s_funcs := s.(s_funcs); s_tables := s.(s_tables); s_mems := s.(s_mems); s_globals := s.(s_globals) ++ [::g] |} ->
+      n = length s.(s_globals) ->
+      pure_reduce hs s locs (HE_wasm_global_create g) hs s' locs (HE_value (HV_wov (WOV_globalref (Mk_globalidx n))))
+  | pr_global_set:
+    forall hs s locs gn idg id s' v g g',
+      hs !! id = Some (HV_wasm_value v) ->
+      hs !! idg = Some (HV_wov (WOV_globalref (Mk_globalidx gn))) ->
+      s.(s_globals) !! gn = Some g ->
+      g.(g_mut) = MUT_mut ->
+      typeof v = typeof (g.(g_val)) ->
+      g' = {|g_mut := MUT_mut; g_val := v|} ->
+      s' = {|s_funcs := s.(s_funcs); s_tables := s.(s_tables); s_mems := s.(s_mems); s_globals := list_insert gn g' s.(s_globals)|} ->
+      pure_reduce hs s locs (HE_wasm_global_set idg id) hs s' locs (HE_value (HV_wasm_value v))
+  | pr_global_get:
+    forall hs s locs idg g gn v,
+      hs !! idg = Some (HV_wov (WOV_globalref (Mk_globalidx gn))) ->
+      g.(g_val) = v ->
+      pure_reduce hs s locs (HE_wasm_global_get idg) hs s locs (HE_value (HV_wasm_value v))
+  (* wasm module expr *)
+   (* TODO: add this back after specifying the concrete host *)
+ (* | pr_compile:
+    forall hs s locs id mo hvl hbytes,
+      hs !! id = Some (HV_list hvl) ->
+      to_bytelist hvl = Some hbytes ->
+      run_parse_module (map byte_of_compcert_byte hbytes) = Some mo -> (* Check: is this correct? *)
+      pure_reduce hs s locs (HE_compile id) hs s locs (HE_value (HV_module mo))*)
+  (* TODO: replace the proxy *)
+  | pr_instantiate:
+    forall hs s locs idm idr mo r rec,
+      hs !! idm = Some (HV_module mo) ->
+      hs !! idr = Some (HV_record r) ->
+      pure_reduce hs s locs (HE_instantiate idm idr) hs s locs rec
+  (* miscellaneous *)
+  | pr_seq_const:
+    forall hs s locs v e,
+      pure_reduce hs s locs (HE_seq (HE_value v) e) hs s locs e
+  | pr_wasm_return:
+    forall hs s locs vs,      
+      pure_reduce hs s locs (HE_wasm_frame (v_to_e_list vs)) hs s locs (HE_value (HV_list (fmap (fun wv => (HV_wasm_value wv)) vs)))
+  | pr_wasm_return_trap:
+      forall hs s locs,
+      pure_reduce hs s locs (HE_wasm_frame ([::AI_trap])) hs s locs (HE_value (HV_trap))
+  | pr_host_return:
+    forall hs s locsf locs ids e vs tn,
+      list_extra.those (fmap (fun id => hs !! id) ids) = Some vs ->
+      pure_reduce hs s locsf (HE_host_frame tn locs (HE_seq (HE_return ids) e)) hs s locsf (HE_value (HV_list vs))
+
+(* TODO: needs all the host_expr reduction steps: compile, instantiate, etc. *)
+(* TODO: needs restructuring to make sense *)
+with wasm_reduce : host_state -> store_record -> datatypes_iris.frame -> list administrative_instruction ->
+                   host_state -> store_record -> datatypes_iris.frame -> list administrative_instruction -> Prop :=
+  | wr_simple :
+      forall e e' s f hs,
+        reduce_simple e e' ->
+        wasm_reduce hs s f e hs s f e'
+
+  (** calling operations **)
+  | wr_call :
+      forall s f i a hs,
+        f.(f_inst).(inst_funcs) !! i = Some a ->
+        wasm_reduce hs s f [::AI_basic (BI_call i)] hs s f [::AI_invoke a]
+  | wr_call_indirect_success :
+      forall s f i a cl tf c hs,
+        stab_addr s f (Wasm_int.nat_of_uint i32m c) = Some a ->
+        s.(s_funcs) !! a = Some cl ->
+        cl_type cl = tf ->
+        stypes s f.(f_inst) i = Some tf ->
+        wasm_reduce hs s f [::AI_basic (BI_const (VAL_int32 c)); AI_basic (BI_call_indirect i)] hs s f [::AI_invoke a]
+  | wr_call_indirect_failure1 :
+      forall s f i a cl tf c hs,
+        stab_addr s f (Wasm_int.nat_of_uint i32m c) = Some a ->
+        s.(s_funcs) !! a = Some cl ->
+        cl_type cl = tf ->
+        stypes s f.(f_inst) i <> Some tf ->
+        wasm_reduce hs s f [::AI_basic (BI_const (VAL_int32 c)); AI_basic (BI_call_indirect i)] hs s f [::AI_trap]
+  | wr_call_indirect_failure2 :
+      forall s f i c hs,
+        stab_addr s f (Wasm_int.nat_of_uint i32m c) = None ->
+        wasm_reduce hs s f [::AI_basic (BI_const (VAL_int32 c)); AI_basic (BI_call_indirect i)] hs s f [::AI_trap]
+  | wr_invoke_native :
+      forall a cl t1s t2s ts es ves vcs n m k zs s f f' i hs,
+        s.(s_funcs) !! a = Some cl ->
+        cl = FC_func_native i (Tf t1s t2s) ts es ->
+        ves = v_to_e_list vcs ->
+        length vcs = n ->
+        length ts = k ->
+        length t1s = n ->
+        length t2s = m ->
+        n_zeros ts = zs ->
+        f'.(f_inst) = i ->
+        f'.(f_locs) = vcs ++ zs ->
+        wasm_reduce hs s f (ves ++ [::AI_invoke a]) hs s f [::AI_local m f' [::AI_basic (BI_block (Tf [::] t2s) es)]]
+  | wr_invoke_host :
+    (* TODO: check *)
+    forall a cl e tf t1s t2s ves vcs m n s s' f hs hs' vs,
+      s.(s_funcs) !! a = Some cl ->
+      cl = FC_func_host tf n e ->
+      tf = Tf t1s t2s ->
+      ves = v_to_e_list vcs ->
+      length vcs = n ->
+      length t1s = n ->
+      length t2s = m ->
+      (* TODO: check if this is what we want *)
+      fmap (fun x => HV_wasm_value x) vcs = vs ->
+      wasm_reduce hs s f (ves ++ [::AI_invoke a]) hs' s' f [::AI_host_frame t1s vs e]
+
+  | wr_host_step :
+    (* TODO: check *)
+    forall hs s (f : datatypes_iris.frame) ts vs e hs' s' vs' e',
+      pure_reduce hs s vs e hs' s' vs' e' ->
+        wasm_reduce hs s f [::AI_host_frame ts vs e] hs' s' f [::AI_host_frame ts vs' e']
+  | wr_host_return :
+    (* TODO: check *)
+    forall hs s f ts vs ids vs' vs'',
+    list_extra.those (fmap (fun id => hs !! id) ids) = Some vs' ->
+    Some vs'' = list_extra.those (fmap (fun x => match x with | HV_wasm_value v => Some v | _ => None end) vs') ->
+    wasm_reduce hs s f [::AI_host_frame ts vs (HE_return ids)] hs s f (v_to_e_list vs'')
+(*  
+  | wr_host_new_host_func :
+    (* TODO: check *)
+    forall hs s f ts vs tf n e idx idx_h hs' s',
+    idx = List.length s.(s_funcs) ->
+    idx_h = List.length hs.(hs_funcs) ->
+    hs' = {| hs_varmap := hs.(hs_varmap); hs_funcs := hs.(hs_funcs) ++ [::e] |} ->
+    s' = {| s_funcs := s.(s_funcs) ++ [::(FC_func_host tf (Mk_funcidx idx_h))]; s_tables := s.(s_tables); s_mems := s.(s_mems); s_globals := s.(s_globals) |} ->
+    wasm_reduce hs s f [::AI_host_frame ts vs (HE_new_host_func tf n e)]
+      hs' s' f [::AI_host_frame ts vs (HE_value (HV_wov (WOV_funcref (Mk_funcidx idx_h))))]
+*)
+  (** get, set, load, and store operations **)
+  | wr_get_local :
+      forall f v j s hs,
+        f.(f_locs) !! j = Some v ->
+        wasm_reduce hs s f [::AI_basic (BI_get_local j)] hs s f [::AI_basic (BI_const v)]
+  | wr_set_local :
+      forall f f' i v s hs,
+        f'.(f_inst) = f.(f_inst) ->
+        f'.(f_locs) = list_insert i v f.(f_locs) ->
+        wasm_reduce hs s f [::AI_basic (BI_const v); AI_basic (BI_set_local i)] hs s f' [::]
+  | wr_get_global :
+      forall s f i v hs,
+        sglob_val s f.(f_inst) i = Some v ->
+        wasm_reduce hs s f [::AI_basic (BI_get_global i)] hs s f [::AI_basic (BI_const v)]
+  | wr_set_global :
+      forall s f i v s' hs,
+        supdate_glob s f.(f_inst) i v = Some s' ->
+        wasm_reduce hs s f [::AI_basic (BI_const v); AI_basic (BI_set_global i)] hs s' f [::]
+  | wr_load_success :
+    forall s i f t bs k a off m hs,
+      smem_ind s f.(f_inst) = Some i ->
+      s.(s_mems) !! i = Some m ->
+      load m (Wasm_int.N_of_uint i32m k) off (t_length t) = Some bs ->
+      wasm_reduce hs s f [::AI_basic (BI_const (VAL_int32 k)); AI_basic (BI_load t None a off)] hs s f [::AI_basic (BI_const (wasm_deserialise bs t))]
+  | wr_load_failure :
+    forall s i f t k a off m hs,
+      smem_ind s f.(f_inst) = Some i ->
+      s.(s_mems) !! i = Some m ->
+      load m (Wasm_int.N_of_uint i32m k) off (t_length t) = None ->
+      wasm_reduce hs s f [::AI_basic (BI_const (VAL_int32 k)); AI_basic (BI_load t None a off)] hs s f [::AI_trap]
+  | wr_load_packed_success :
+    forall s i f t tp k a off m bs sx hs,
+      smem_ind s f.(f_inst) = Some i ->
+      s.(s_mems) !! i = Some m ->
+      load_packed sx m (Wasm_int.N_of_uint i32m k) off (tp_length tp) (t_length t) = Some bs ->
+      wasm_reduce hs s f [::AI_basic (BI_const (VAL_int32 k)); AI_basic (BI_load t (Some (tp, sx)) a off)] hs s f [::AI_basic (BI_const (wasm_deserialise bs t))]
+  | wr_load_packed_failure :
+    forall s i f t tp k a off m sx hs,
+      smem_ind s f.(f_inst) = Some i ->
+      s.(s_mems) !! i = Some m ->
+      load_packed sx m (Wasm_int.N_of_uint i32m k) off (tp_length tp) (t_length t) = None ->
+      wasm_reduce hs s f [::AI_basic (BI_const (VAL_int32 k)); AI_basic (BI_load t (Some (tp, sx)) a off)] hs s f [::AI_trap]
+  | wr_store_success :
+    forall t v s i f mem' k a off m hs,
+      types_agree t v ->
+      smem_ind s f.(f_inst) = Some i ->
+      s.(s_mems) !! i = Some m ->
+      store m (Wasm_int.N_of_uint i32m k) off (bits v) (t_length t) = Some mem' ->
+      wasm_reduce hs s f [::AI_basic (BI_const (VAL_int32 k)); AI_basic (BI_const v); AI_basic (BI_store t None a off)] hs (upd_s_mem s (update_list_at s.(s_mems) i mem')) f [::]
+  | wr_store_failure :
+    forall t v s i f m k off a hs,
+      types_agree t v ->
+      smem_ind s f.(f_inst) = Some i ->
+      s.(s_mems) !! i = Some m ->
+      store m (Wasm_int.N_of_uint i32m k) off (bits v) (t_length t) = None ->
+      wasm_reduce hs s f [::AI_basic (BI_const (VAL_int32 k)); AI_basic (BI_const v); AI_basic (BI_store t None a off)] hs s f [::AI_trap]
+  | wr_store_packed_success :
+    forall t v s i f m k off a mem' tp hs,
+      types_agree t v ->
+      smem_ind s f.(f_inst) = Some i ->
+      s.(s_mems) !! i = Some m ->
+      store_packed m (Wasm_int.N_of_uint i32m k) off (bits v) (tp_length tp) = Some mem' ->
+      wasm_reduce hs s f [::AI_basic (BI_const (VAL_int32 k)); AI_basic (BI_const v); AI_basic (BI_store t (Some tp) a off)] hs (upd_s_mem s (update_list_at s.(s_mems) i mem')) f [::]
+  | wr_store_packed_failure :
+    forall t v s i f m k off a tp hs,
+      types_agree t v ->
+      smem_ind s f.(f_inst) = Some i ->
+      s.(s_mems) !! i = Some m ->
+      store_packed m (Wasm_int.N_of_uint i32m k) off (bits v) (tp_length tp) = None ->
+      wasm_reduce hs s f [::AI_basic (BI_const (VAL_int32 k)); AI_basic (BI_const v); AI_basic (BI_store t (Some tp) a off)] hs s f [::AI_trap]
+
+  (** memory **)
+  | wr_current_memory :
+    forall i f m n s hs,
+      smem_ind s f.(f_inst) = Some i ->
+      s.(s_mems) !! i = Some m ->
+      mem_size m = n ->
+      wasm_reduce hs s f [::AI_basic (BI_current_memory)] hs s f [::AI_basic (BI_const (VAL_int32 (Wasm_int.int_of_Z i32m (Z.of_N n))))]
+  | wr_grow_memory_success :
+    forall s i f m n mem' c hs,
+      smem_ind s f.(f_inst) = Some i ->
+      s.(s_mems) !! i = Some m ->
+      mem_size m = n ->
+      mem_grow m (Wasm_int.N_of_uint i32m c) = Some mem' ->
+      wasm_reduce hs s f [::AI_basic (BI_const (VAL_int32 c)); AI_basic BI_grow_memory] hs (upd_s_mem s (update_list_at s.(s_mems) i mem')) f [::AI_basic (BI_const (VAL_int32 (Wasm_int.int_of_Z i32m (Z.of_N n))))]
+  | wr_grow_memory_failure :
+    forall i f m n s c hs,
+      smem_ind s f.(f_inst) = Some i ->
+      s.(s_mems) !!i = Some m ->
+      mem_size m = n ->
+      wasm_reduce hs s f [::AI_basic (BI_const (VAL_int32 c)); AI_basic BI_grow_memory] hs s f [::AI_basic (BI_const (VAL_int32 int32_minus_one))]
+
+  (** label and local **)
+  | wr_label :
+    forall s f es les s' f' es' les' k lh hs hs',
+      wasm_reduce hs s f es hs' s' f' es' ->
+      lfilled k lh es les ->
+      lfilled k lh es' les' ->
+      wasm_reduce hs s f les hs' s' f' les'
+  | wr_local :
+    forall s f es s' f' es' n f0 hs hs',
+      wasm_reduce hs s f es hs' s' f' es' ->
+      wasm_reduce hs s f0 [::AI_local n f es] hs' s' f0 [::AI_local n f' es']
+.
+
+Inductive head_reduce: state -> iris_expr -> state -> iris_expr -> Prop :=
+  | purer_headr:
+    forall hs s locs e hs' s' locs' e',
+      pure_reduce hs s locs e hs' s' locs' e' ->
+      head_reduce (hs, s, locs) e (hs', s', locs') e'.
+
+Definition head_step (e : iris_expr) (s : state) (os : list observation) (e' : iris_expr) (s' : state) (es' : list iris_expr) : Prop :=
+  head_reduce s e s' e' /\
+  os = nil /\
+  es' = nil. (* ?? *)
+
+Lemma head_step_not_val: forall e1 σ1 κ e2 σ2 efs,
+  head_step e1 σ1 κ e2 σ2 efs ->
+  to_val e1 = None.
+Proof.
+  move => e1 σ1 κ e2 σ2 efs H.
+  destruct H as [HR _].
+  inversion HR as [hs s locs e hs' s' locs' e' H]; subst.
+  by inversion H.
+Qed.
 
 Lemma wasm_mixin : LanguageMixin of_val to_val head_step.
 Proof.
@@ -63,20 +699,22 @@ Class wglobG Σ := WGlobG {
   glob_gen_hsG :> gen_heapG N global Σ;
 }.
 
-Instance heapG_irisG `{hsG Σ, locG Σ, wfuncG Σ, wtabG Σ, wmemG Σ, wglobG Σ} : irisG wasm_lang Σ := {
+Instance heapG_irisG `{!hsG Σ, !locG Σ, !wfuncG Σ, !wtabG Σ, !wmemG Σ, !wglobG Σ} : irisG wasm_lang Σ := {
   iris_invG := hs_invG; (* TODO: determine the correct invariant. Or, do we have any actually? *)
-  state_interp σ κs _ :=
+  state_interp σ _ κs _ :=
     let (hss, locs) := σ in
     let (hs, s) := hss in
-    ((gen_heap_ctx hs) ∗
-      (gen_heap_ctx (gmap_of_list locs)) ∗
-      (gen_heap_ctx (gmap_of_list s.(s_funcs))) ∗
-      (gen_heap_ctx (gmap_of_list s.(s_tables))) ∗
-      (gen_heap_ctx (gmap_of_mem s.(s_mems))) ∗
-      (gen_heap_ctx (gmap_of_list s.(s_globals)))
+    ((gen_heap_interp hs) ∗
+      (gen_heap_interp (gmap_of_list locs)) ∗
+      (gen_heap_interp (gmap_of_list s.(s_funcs))) ∗
+      (gen_heap_interp (gmap_of_list s.(s_tables))) ∗
+      (gen_heap_interp (gmap_of_mem s.(s_mems))) ∗
+      (gen_heap_interp (gmap_of_list s.(s_globals)))
     )%I;
   fork_post _ := True%I;
-                                                                                                  }.
+  num_laters_per_step := (fun x => 0); (* TODO: weird, but makes this compile *)
+  state_interp_mono _ _ _ _ := fupd_intro _ _
+}.
 
 (* This means the proposition that 'the location l of the heap has value v, and we own q of it' 
      (fractional algebra). 
